redefine safety property

src/Safety.v
@@ -2,16 +2,71 @@ Require Import Gc.Language Gc.Gc.
 
 Require Import List ListSet Equality CpdtTactics.
 
+Ltac destructo :=
+  repeat match goal with
+         | [H : _ /\ _ |- _] => destruct H
+         | [H : exists _, _|- _] => destruct H
+         | [H : _ <-> _ |- _] => destruct H
+         end.
+
+
+Definition struct_equiv (s1: list val) (s2: list val) : Prop :=
+  length s1 = length s2
+  /\
+  forall n i,
+    nth_error s1 n = Some (Int i) <-> nth_error s2 n = Some (Int i).
+
+Lemma struct_equiv_refl : forall s1, struct_equiv s1 s1.
+Proof.
+  Hint Unfold struct_equiv.
+  induction s1 ; crush.
+Qed.
+Hint Resolve struct_equiv_refl.
+
+Lemma struct_equiv_symm : forall s1 s2, struct_equiv s1 s2 -> struct_equiv s2 s1.
+Proof.
+  Hint Unfold struct_equiv.
+  intros.
+  unfold struct_equiv in *.
+  destructo.
+  split. auto.
+  intros.
+  specialize (H0 n i).
+  destructo.
+  split ; auto.
+Qed.
+Hint Resolve struct_equiv_symm.
+
+Lemma struct_equiv_trans : forall s1 s2 s3,
+    struct_equiv s1 s2 ->
+    struct_equiv s2 s3 ->
+    struct_equiv s1 s3.
+Proof.
+  Hint Unfold struct_equiv.
+  intros.
+  unfold struct_equiv in *.
+  destructo.
+  split. crush.
+  intros.
+  specialize (H1 n i).
+  specialize (H2 n i).
+  destructo.
+  split ; auto.
+Qed.
+Hint Resolve struct_equiv_trans.
+
+
 (* All integers reachable from the same variable, address, and index. *)
 Definition equiv' (s1 s2: state) : Prop :=
-  forall v p1 address p1' k i,
+  forall v p1 address p1' struct1,
       roots_maps (roots s1) v p1 ->
       addresses (heap s1) p1 address p1' ->
-      heap_maps (heap s1) p1' k (Int i) ->
-      exists p2 p2',
+      heap_maps_struct (heap s1) p1' struct1 ->
+      exists p2 p2' struct2,
         roots_maps (roots s2) v p2 /\
         addresses (heap s2) p2 address p2' /\
-        heap_maps (heap s2) p2' k (Int i).
+        heap_maps_struct (heap s2) p2' struct2 /\
+        struct_equiv struct1 struct2.
 
 Definition equiv (s1 s2: state) : Prop :=
   (output s1 = output s2) /\ equiv' s1 s2 /\ equiv' s2 s1.
@@ -23,7 +78,7 @@ Lemma equiv_refl : forall s1, equiv s1 s1.
   split ;
     unfold equiv' ;
     intros ;
-    exists p1, p1';
+    exists p1, p1', struct1 ;
     auto.
 Qed.
 
@@ -33,12 +88,6 @@ Lemma equiv_symm : forall s1 s2, equiv s1 s2 -> equiv s2 s1.
   crush.
 Qed.
 
-Ltac destructo :=
-  repeat match goal with
-         | [H : _ /\ _ |- _] => destruct H
-         | [H : exists _, _|- _] => destruct H
-         end.
-
 Lemma equiv_trans : forall s1 s2 s3, equiv s1 s2 -> equiv s2 s3 -> equiv s1 s3.
 Proof.
   intros.
@@ -47,20 +96,22 @@ Proof.
   split. crush.
   clear H H0.
   split ; unfold equiv' ; intros.
-  * specialize (H3 v p1 address p1' k i).
+  * specialize (H3 v p1 address p1' struct1).
     intuition.
     destructo.
-    eapply H1.
-    apply H3.
-    apply H6.
-    apply H7.
-  * specialize (H2 v p1 address p1' k i).
+    specialize (H1 v x address x0 x1).
     intuition.
     destructo.
-    eapply H4.
-    apply H2.
-    apply H6.
-    apply H7.
+    exists x2, x3, x4.
+    eauto.
+  * specialize (H2 v p1 address p1' struct1).
+    intuition.
+    destructo.
+    specialize (H4 v x address x0 x1).
+    intuition.
+    destructo.
+    exists x2, x3, x4.
+    eauto.
 Qed.
 
 Theorem gc_forward_safety :
@@ -71,19 +122,21 @@ Proof.
   intros.
   exists p1.
   exists p1'.
+  exists struct1.
   intuition.
   * subst; eapply pointer_equivalence; eauto.
-  * specialize (heap_maps_implies_heap_get _ _ _ _ H1); intros.
-    destruct H2; inversion H2; clear H2.
+  * (* specialize (heap_maps_implies_heap_get _ _ _ _ H1); intros. *)
+    unfold heap_maps_struct in H1.
     specialize address_maps_to_value with (heap (gc st)) p1 p1' address; intros.
     assert (addresses (heap (gc st)) p1 address p1').
     - subst; eapply pointer_equivalence; eauto.
-    - eapply H2 in H5.
-      destruct H5.
-      assert (x = x0).
-      + eapply (value_equivalence (roots st) (heap st) (heap (gc st)) p1' x x0); crush.
-      + destruct H6.
-        eapply heap_get_implies_heap_maps; crush.
+    - intuition.
+      destructo.
+      assert (heap_maps_struct (heap st) p1' struct1). auto.
+      assert (struct1 = x).
+      + eapply (value_equivalence (roots st) (heap st) (heap (gc st)) p1' struct1 x); crush.
+      + subst.
+        auto.
 Qed.
 
 Theorem gc_backward_safety :
